Incorrect, but extracting and running-ish for sha

examples/primitives/ml/test_sha256.ml
@@ -1,6 +1,24 @@
+open Char
+open SBuffer
+open FStar_SBytes
 open Crypto_Sha256
 
+let from_string s =
+  let b = create 0 (String.length s) in
+  for i = 0 to (String.length s - 1) do
+    upd b i (code (String.get s i))
+  done;
+  b
+
+let from_bytestring s =
+  let b = create 0 ((String.length s) / 2) in
+  for i = 0 to ((String.length s / 2) - 1) do
+    upd b i (int_of_string ("0x" ^ (String.sub s (2*i) 2)))
+  done;
+  b
+
 let _ =
+  let hash = create (0) 32 in
   let input = [ "abc";
                 "abcabc";
                 "abcdefghijklmnopqrstuvwxyz";
@@ -11,7 +29,9 @@ let _ =
   List.iter (
       fun e ->
       Printf.printf "INPUT : %s\n" e;
-      sha256 (Bytes.of_string e) (String.length e)
+      sha256 hash (from_string e) (String.length e);
+      print_bytes hash
     ) input;
   Printf.printf "INPUT : 1 million de 'a'\n";
-  sha256 (Bytes.make 1000000 '\x61') 1000000
+  sha256 hash (from_string (Bytes.make 1000000 '\x61')) 1000000;
+  print_bytes hash
